specs/lib/fst/Spec.Lib.IntTypes.fst
@@ -7,7 +7,9 @@ let pow2_values n =
     assert_norm (pow2 0 = 1);
     assert_norm (pow2 8 = 0x100);
     assert_norm (pow2 16 = 0x10000);
+    assert_norm (pow2 24 = 0x1000000);
     assert_norm (pow2 32 = 0x100000000);
+    assert_norm (pow2 48 = 0x1000000000000);
     assert_norm (pow2 64 = 0x10000000000000000);
     assert_norm (pow2 128 = 0x100000000000000000000000000000000)
 
@@ -15,7 +17,9 @@ let uint_t (t:inttype) : Type0 =
   match t with
   | U8 -> UInt8.t
   | U16 -> UInt16.t
+  | U24 -> UInt32.t
   | U32 -> UInt32.t
+  | U48 -> UInt64.t
   | U64 -> UInt64.t
   | U128 -> UInt128.t
   | SIZE -> UInt32.t
@@ -25,14 +29,16 @@ let uint_to_nat_ #t (x:uint_t t) =
   match t with
   | U8 -> UInt8.v x
   | U16 -> UInt16.v x
+  | U24 -> UInt32.v x
   | U32 -> UInt32.v x
+  | U48 -> UInt64.v x
   | U64 -> UInt64.v x
   | U128 -> UInt128.v x
   | SIZE -> UInt32.v x
 
 let uint_v #t u = uint_to_nat_ u
 
-(* Declared in .fsti: uint8, uint16, uint32, uint64, uint128 *)
+(* Declared in .fsti: uint8, uint16, uint24, uint32, uint48, uint64, uint128 *)
 
 let u8 x : uint8  = UInt8.uint_to_t x
 
@@ -40,9 +46,17 @@ let u16 x : uint16 = UInt16.uint_to_t x
 
 let u16_us x = x
 
+let u24 x : uint24 = UInt32.uint_to_t x
+
+let u24_ul x = x
+
 let u32 x : uint32 = UInt32.uint_to_t x
 
 let u32_ul x = x
+
+let u48 x : uint48 = UInt64.uint_to_t x
+
+let u48_uL x = x
 
 let u64 x : uint64 = UInt64.uint_to_t x
 
@@ -59,7 +73,9 @@ let nat_to_uint #t x : uint_t t =
   match t with
   | U8 -> u8 x
   | U16 -> u16 x
+  | U24 -> u24 x
   | U32 -> u32 x
+  | U48 -> u48 x
   | U64 -> u64 x
   | U128 -> u128 x
   | SIZE -> size_ x
@@ -69,35 +85,67 @@ let cast #t t' u  =
   match t, t' with
   | U8, U8 -> u
   | U8, U16 -> FStar.Int.Cast.uint8_to_uint16 u
+  | U8, U24 -> FStar.Int.Cast.uint8_to_uint32 u
   | U8, U32 -> FStar.Int.Cast.uint8_to_uint32 u
+  | U8, U48 -> FStar.Int.Cast.uint8_to_uint64 u
   | U8, U64 -> FStar.Int.Cast.uint8_to_uint64 u
   | U8, U128 -> FStar.UInt128.uint64_to_uint128 (FStar.Int.Cast.uint8_to_uint64 u)
+
   | U16, U8 -> FStar.Int.Cast.uint16_to_uint8 u
   | U16, U16 -> u
+  | U16, U24 -> FStar.Int.Cast.uint16_to_uint32 u
   | U16, U32 -> FStar.Int.Cast.uint16_to_uint32 u
+  | U16, U48 -> FStar.Int.Cast.uint16_to_uint64 u
   | U16, U64 -> FStar.Int.Cast.uint16_to_uint64 u
   | U16, U128 -> FStar.UInt128.uint64_to_uint128 (FStar.Int.Cast.uint16_to_uint64 u)
+
+  | U24, U8 -> FStar.Int.Cast.uint32_to_uint8 u
+  | U24, U16 -> FStar.Int.Cast.uint32_to_uint16 u
+  | U24, U24 -> u
+  | U24, U32 -> u
+  | U24, U48 -> FStar.Int.Cast.uint32_to_uint64 u
+  | U24, U64 -> FStar.Int.Cast.uint32_to_uint64 u
+  | U24, U128 -> FStar.UInt128.uint64_to_uint128 (FStar.Int.Cast.uint32_to_uint64 u)
+
   | U32, U8 -> FStar.Int.Cast.uint32_to_uint8 u
   | U32, U16 -> FStar.Int.Cast.uint32_to_uint16 u
+  | U32, U24 -> u
   | U32, U32 -> u
+  | U32, U48 -> FStar.Int.Cast.uint32_to_uint64 u
   | U32, U64 -> FStar.Int.Cast.uint32_to_uint64 u
   | U32, U128 -> FStar.UInt128.uint64_to_uint128 (FStar.Int.Cast.uint32_to_uint64 u)
+
+  | U48, U8 -> FStar.Int.Cast.uint64_to_uint8 u
+  | U48, U16 -> FStar.Int.Cast.uint64_to_uint16 u
+  | U48, U24 -> FStar.Int.Cast.uint64_to_uint32 u
+  | U48, U32 -> FStar.Int.Cast.uint64_to_uint32 u
+  | U48, U48 -> u
+  | U48, U64 -> u
+  | U64, U128 -> FStar.UInt128.uint64_to_uint128 u
+
   | U64, U8 -> FStar.Int.Cast.uint64_to_uint8 u
   | U64, U16 -> FStar.Int.Cast.uint64_to_uint16 u
+  | U64, U24 -> FStar.Int.Cast.uint64_to_uint32 u
   | U64, U32 -> FStar.Int.Cast.uint64_to_uint32 u
+  | U64, U48 -> u
   | U64, U64 -> u
   | U64, U128 -> FStar.UInt128.uint64_to_uint128 u
-  | U128, U64 -> FStar.UInt128.uint128_to_uint64 u
+
   | U128, U8 -> FStar.Int.Cast.uint64_to_uint8 (FStar.UInt128.uint128_to_uint64 u)
   | U128, U16 -> FStar.Int.Cast.uint64_to_uint16 (FStar.UInt128.uint128_to_uint64 u)
+  | U128, U24 -> FStar.Int.Cast.uint64_to_uint32 (FStar.UInt128.uint128_to_uint64 u)
   | U128, U32 -> FStar.Int.Cast.uint64_to_uint32 (FStar.UInt128.uint128_to_uint64 u)
+  | U128, U48 -> FStar.UInt128.uint128_to_uint64 u
+  | U128, U64 -> FStar.UInt128.uint128_to_uint64 u
   | U128, U128 -> u
 
 let add_mod #t a b =
   match t with
   | U8  -> (UInt8.add_mod a b)
   | U16 -> (UInt16.add_mod a b)
+  | U24 -> (UInt32.add_mod a b)
   | U32 -> (UInt32.add_mod a b)
+  | U48 -> (UInt64.add_mod a b)
   | U64 -> (UInt64.add_mod a b)
   | U128 -> (UInt128.add_mod a b)
   | SIZE -> (UInt32.add_mod a b)
@@ -107,7 +155,9 @@ let add #t a b =
   match t with
   | U8 -> (UInt8.add a b)
   | U16 -> (UInt16.add a b)
+  | U24 -> (UInt32.add a b)
   | U32 -> (UInt32.add a b)
+  | U48 -> (UInt64.add a b)
   | U64 -> (UInt64.add a b)
   | U128 -> (UInt128.add a b)
   | SIZE -> (UInt32.add a b)
@@ -116,27 +166,30 @@ let incr #t a =
   match t with
   | U8 -> (UInt8.add a 0x1uy)
   | U16 -> (UInt16.add a 0x1us)
+  | U24 -> (UInt32.add a 0x1ul)
   | U32 -> (UInt32.add a 0x1ul)
+  | U48 -> (UInt64.add a 0x1uL)
   | U64 -> (UInt64.add a 0x1uL)
   | U128 -> (UInt128.add a (UInt128.uint_to_t 1))
   | SIZE -> (UInt32.add a 0x1ul)
-
-
 
 let mul_mod #t a b =
   match t with
   | U8 -> (UInt8.mul_mod a b)
   | U16 -> (UInt16.mul_mod a b)
+  | U24 -> (UInt32.mul_mod a b)
   | U32 -> (UInt32.mul_mod a b)
+  | U48 -> (UInt64.mul_mod a b)
   | U64 -> (UInt64.mul_mod a b)
   | SIZE -> (UInt32.mul_mod a b)
-
 
 let mul #t a b =
   match t with
   | U8 -> (UInt8.mul a b)
   | U16 -> (UInt16.mul a b)
+  | U24 -> (UInt32.mul a b)
   | U32 -> (UInt32.mul a b)
+  | U48 -> (UInt64.mul a b)
   | U64 -> (UInt64.mul a b)
   | SIZE -> (UInt32.mul a b)
 
@@ -146,7 +199,9 @@ let sub_mod #t a b =
   match t with
   | U8 -> (UInt8.sub_mod a b)
   | U16 -> (UInt16.sub_mod a b)
+  | U24 -> (UInt32.sub_mod a b)
   | U32 -> (UInt32.sub_mod a b)
+  | U48 -> (UInt64.sub_mod a b)
   | U64 -> (UInt64.sub_mod a b)
   | U128 -> (UInt128.sub_mod a b)
   | SIZE -> (UInt32.sub_mod a b)
@@ -156,7 +211,9 @@ let sub #t a b =
   match t with
   | U8 -> (UInt8.sub a b)
   | U16 -> (UInt16.sub a b)
+  | U24 -> (UInt32.sub a b)
   | U32 -> (UInt32.sub a b)
+  | U48 -> (UInt64.sub a b)
   | U64 -> (UInt64.sub a b)
   | U128 -> (UInt128.sub a b)
   | SIZE -> (UInt32.sub a b)
@@ -165,7 +222,9 @@ let decr #t a =
   match t with
   | U8 -> (UInt8.sub a 0x1uy)
   | U16 -> (UInt16.sub a 0x1us)
+  | U24 -> (UInt32.sub a 0x1ul)
   | U32 -> (UInt32.sub a 0x1ul)
+  | U48 -> (UInt64.sub a 0x1uL)
   | U64 -> (UInt64.sub a 0x1uL)
   | U128 -> (UInt128.sub a (UInt128.uint_to_t 1))
   | SIZE -> (UInt32.sub a 0x1ul)
@@ -174,7 +233,9 @@ let logxor #t a b =
   match t with
   | U8 -> (UInt8.logxor a b)
   | U16 -> (UInt16.logxor a b)
+  | U24 -> (UInt32.logxor a b)
   | U32 -> (UInt32.logxor a b)
+  | U48 -> (UInt64.logxor a b)
   | U64 -> (UInt64.logxor a b)
   | U128 -> (UInt128.logxor a b)
   | SIZE -> (UInt32.logxor a b)
@@ -184,7 +245,9 @@ let logand #t a b =
   match t with
   | U8 -> (UInt8.logand a b)
   | U16 -> (UInt16.logand a b)
+  | U24 -> (UInt32.logand a b)
   | U32 -> (UInt32.logand a b)
+  | U48 -> (UInt64.logand a b)
   | U64 -> (UInt64.logand a b)
   | U128 -> (UInt128.logand a b)
   | SIZE -> (UInt32.logand a b)
@@ -194,7 +257,9 @@ let logor #t a b =
   match t with
   | U8 -> (UInt8.logor a b)
   | U16 -> (UInt16.logor a b)
+  | U24 -> (UInt32.logor a b)
   | U32 -> (UInt32.logor a b)
+  | U48 -> (UInt64.logor a b)
   | U64 -> (UInt64.logor a b)
   | U128 -> (UInt128.logor a b)
   | SIZE -> (UInt32.logor a b)
@@ -204,17 +269,20 @@ let lognot #t a =
   match t with
   | U8 -> (UInt8.lognot a)
   | U16 -> (UInt16.lognot a)
+  | U24 -> (UInt32.lognot a)
   | U32 -> (UInt32.lognot a)
+  | U48 -> (UInt64.lognot a)
   | U64 -> (UInt64.lognot a)
   | U128 -> (UInt128.lognot a)
   | SIZE -> (UInt32.lognot a)
-
 
 let shift_right #t a b =
   match t with
   | U8 -> (UInt8.shift_right a b)
   | U16 -> (UInt16.shift_right a b)
+  | U24 -> (UInt32.shift_right a b)
   | U32 -> (UInt32.shift_right a b)
+  | U48 -> (UInt64.shift_right a b)
   | U64 -> (UInt64.shift_right a b)
   | U128 -> (UInt128.shift_right a b)
   | SIZE -> (UInt32.shift_right a b)
@@ -223,11 +291,12 @@ let shift_left #t a b =
   match t with
   | U8 -> (UInt8.shift_left a b)
   | U16 -> (UInt16.shift_left a b)
+  | U24 -> (UInt32.shift_left a b)
   | U32 -> (UInt32.shift_left a b)
+  | U48 -> (UInt64.shift_left a b)
   | U64 -> (UInt64.shift_left a b)
   | U128 -> (UInt128.shift_left a b)
   | SIZE -> (UInt32.shift_left a b)
-
 
 let rotate_right #t a b =
   (logor (shift_right a b)  (shift_left a (sub #U32 (u32 (bits t)) b)))
@@ -239,7 +308,9 @@ let eq_mask #t a b =
   match t with
   | U8 -> if FStar.UInt8.(a =^ b) then (u8 (maxint U8)) else (u8 0)
   | U16 -> if FStar.UInt16.(a =^ b) then (u16 (maxint U16)) else (u16 0)
+  | U24 -> if FStar.UInt32.(a =^ b) then (u24 (maxint U24)) else (u24 0)
   | U32 -> if FStar.UInt32.(a =^ b) then (u32 (maxint U32)) else (u32 0)
+  | U48 -> if FStar.UInt64.(a =^ b) then (u48 (maxint U48)) else (u48 0)
   | U64 -> if FStar.UInt64.(a =^ b) then (u64 (maxint U64)) else (u64 0)
   | U128 -> if FStar.UInt128.(a =^ b) then (u128 (maxint U128)) else (u128 0)
   | SIZE -> if FStar.UInt32.(a =^ b) then (u32 (maxint U32)) else (u32 0)
@@ -248,7 +319,9 @@ let neq_mask #t a b =
   match t with
   | U8 -> if not FStar.UInt8.(a =^ b) then (u8 (maxint U8)) else (u8 0)
   | U16 -> if not FStar.UInt16.(a =^ b) then (u16 (maxint U16)) else (u16 0)
+  | U24 -> if not FStar.UInt32.(a =^ b) then (u24 (maxint U24)) else (u24 0)
   | U32 -> if not FStar.UInt32.(a =^ b) then (u32 (maxint U32)) else (u32 0)
+  | U64 -> if not FStar.UInt64.(a =^ b) then (u48 (maxint U48)) else (u48 0)
   | U64 -> if not FStar.UInt64.(a =^ b) then (u64 (maxint U64)) else (u64 0)
   | U128 -> if not FStar.UInt128.(a =^ b) then (u128 (maxint U128)) else (u128 0)
   | SIZE -> if not FStar.UInt32.(a =^ b) then (u32 (maxint U32)) else (u32 0)
@@ -257,7 +330,9 @@ let gt_mask #t a b =
   match t with
   | U8 -> if FStar.UInt8.(a >^ b) then (u8 (maxint U8)) else (u8 0)
   | U16 -> if FStar.UInt16.(a >^ b) then (u16 (maxint U16)) else (u16 0)
+  | U24 -> if FStar.UInt32.(a >^ b) then (u24 (maxint U24)) else (u24 0)
   | U32 -> if FStar.UInt32.(a >^ b) then (u32 (maxint U32)) else (u32 0)
+  | U48 -> if FStar.UInt64.(a >^ b) then (u48 (maxint U48)) else (u48 0)
   | U64 -> if FStar.UInt64.(a >^ b) then (u64 (maxint U64)) else (u64 0)
   | U128 -> if FStar.UInt128.(a >^ b) then (u128 (maxint U128)) else (u128 0)
   | SIZE -> if FStar.UInt32.(a >^ b) then (u32 (maxint U32)) else (u32 0)
@@ -266,7 +341,9 @@ let gte_mask #t a b =
   match t with
   | U8 -> if FStar.UInt8.(a >=^ b) then (u8 (maxint U8)) else (u8 0)
   | U16 -> if FStar.UInt16.(a >=^ b) then (u16 (maxint U16)) else (u16 0)
+  | U48 -> if FStar.UInt32.(a >=^ b) then (u48 (maxint U48)) else (u48 0)
   | U32 -> if FStar.UInt32.(a >=^ b) then (u32 (maxint U32)) else (u32 0)
+  | U48 -> if FStar.UInt64.(a >=^ b) then (u48 (maxint U48)) else (u48 0)
   | U64 -> if FStar.UInt64.(a >=^ b) then (u64 (maxint U64)) else (u64 0)
   | U128 -> if FStar.UInt128.(a >=^ b) then (u128 (maxint U128)) else (u128 0)
   | SIZE -> if FStar.UInt32.(a >=^ b) then (u32 (maxint U32)) else (u32 0)
@@ -275,7 +352,9 @@ let lt_mask #t a b =
   match t with
   | U8 -> if FStar.UInt8.(a <^ b) then (u8 (maxint U8)) else (u8 0)
   | U16 -> if FStar.UInt16.(a <^ b) then (u16 (maxint U16)) else (u16 0)
+  | U24 -> if FStar.UInt32.(a <^ b) then (u24 (maxint U24)) else (u24 0)
   | U32 -> if FStar.UInt32.(a <^ b) then (u32 (maxint U32)) else (u32 0)
+  | U48 -> if FStar.UInt64.(a <^ b) then (u48 (maxint U48)) else (u48 0)
   | U64 -> if FStar.UInt64.(a <^ b) then (u64 (maxint U64)) else (u64 0)
   | U128 -> if FStar.UInt128.(a <^ b) then (u128 (maxint U128)) else (u128 0)
   | SIZE -> if FStar.UInt32.(a <^ b) then (u32 (maxint U32)) else (u32 0)
@@ -284,7 +363,9 @@ let lte_mask #t a b =
   match t with
   | U8 -> if FStar.UInt8.(a <=^ b) then (u8 (maxint U8)) else (u8 0)
   | U16 -> if FStar.UInt16.(a <=^ b) then (u16 (maxint U16)) else (u16 0)
+  | U24 -> if FStar.UInt32.(a <=^ b) then (u24 (maxint U24)) else (u24 0)
   | U32 -> if FStar.UInt32.(a <=^ b) then (u32 (maxint U32)) else (u32 0)
+  | U48 -> if FStar.UInt64.(a <=^ b) then (u48 (maxint U48)) else (u48 0)
   | U64 -> if FStar.UInt64.(a <=^ b) then (u64 (maxint U64)) else (u64 0)
   | U128 -> if FStar.UInt128.(a <=^ b) then (u128 (maxint U128)) else (u128 0)
   | SIZE -> if FStar.UInt32.(a <=^ b) then (u32 (maxint U32)) else (u32 0)
