specs/lib/fst/Spec.Lib.RawIntTypes.fst
@@ -11,7 +11,11 @@ let u8_from_UInt8 x = x
 
 let u16_from_UInt16 x = x
 
+let u24_from_UInt32 x = x
+
 let u32_from_UInt32 x = x
+
+let u48_from_UInt64 x = x
 
 let u64_from_UInt64 x = x
 
@@ -23,7 +27,11 @@ let u8_to_UInt8 x = x
 
 let u16_to_UInt16 x = x
 
+let u24_to_UInt32 x = x
+
 let u32_to_UInt32 x = x
+
+let u48_to_UInt64 x = x
 
 let u64_to_UInt64 x = x
 
@@ -35,7 +43,9 @@ let uint_to_nat #t (x:uint_t t) =
   match t with
   | U8 -> UInt8.v x
   | U16 -> UInt16.v x
+  | U24 -> UInt32.v x
   | U32 -> UInt32.v x
+  | U48 -> UInt64.v x
   | U64 -> UInt64.v x
   | U128 -> UInt128.v x
   | SIZE -> UInt32.v x
